custom array index syntax and LoadWord lw case cleanup

SP1Chips/Load/LoadWord.lean
@@ -5,11 +5,57 @@ import LeanRV64IM.Specialization
 import LeanRV64IM.RiscvMem
 import LeanRV64IM.RiscvInstsEnd
 
+syntax:max term noWs "[" withoutPosition(term) "]$" : term
+macro_rules | `($x[$i]$) => `(getElem $x $i (by simp))
+
 open LeanRV64IM.Functions
+
+lemma Sail.run_writeReg_no_run (reg : Register) (v : RegisterType reg) :
+    (Sail.writeReg reg v) s =
+      .ok PUnit.unit { s with regs := s.regs.insert reg v} := rfl
+
+namespace Sail
+
+lemma run_write_reg_no_run (idx : BitVec 5) (val : BitVec 64) :
+    (write_reg idx val) =
+      let reg : Register := reg_idx_to_Register idx
+      if idx = 0#5 then if val = 0#64 then pure () else throw Sail.Error.Unreachable
+        else Sail.writeReg reg (bitVecToRegidxVal idx val) := by
+  unfold write_reg; aesop
+
+end Sail
+
+namespace BitVec
+
+set_option maxHeartbeats 4000000 in
+theorem u64_limbs_add_is_append {x y z a : ℕ}
+  (hx : x < 65536)
+  (hy : y < 65536)
+  (hz : z < 65536)
+  (ha : a < 65536)
+  : BitVec.ofNat 64 (x + y <<< 16 + z <<< 32 + a <<< 48)
+  = (BitVec.ofNatLT (w := 16) a ha)
+    ++ (BitVec.ofNatLT (w := 16) z hz)
+    ++ (BitVec.ofNatLT (w := 16) y hy)
+    ++ (BitVec.ofNatLT (w := 16) x hx)
+  := by
+    -- rw [←BitVec.ofNatLT_eq_ofNat (by simp [Nat.shiftLeft_eq]; omega)]
+    -- rw [BitVec.append_def]
+    -- rw [BitVec.append_def]
+    -- rw [BitVec.append_def]
+    -- simp [BitVec.shiftLeftZeroExtend]
+    -- unfold BitVec.setWidth
+    -- simp only [Nat.reduceLeDiff, ↓reduceDIte]
+    -- unfold BitVec.setWidth'
+    sorry
+
+end BitVec
 
 namespace Load
 
 namespace LoadWord
+
+open BitVec
 
 instance : ReflBEq Privilege where
   rfl := by
@@ -68,13 +114,17 @@ def sp1_lw : SailM ExecutionResult :=
   do
     let op_a := sp1_op_a Main cstrs h_is_lw
     Sail.writeReg Register.nextPC (Word.toBitVec64 #v[Main[3] + 4, Main[4], Main[5], 0])
-    Sail.write_reg op_a (Word.toBitVec64 #v[Main[39], Main[40], Main[41] * 65536, Main[41] * 65536])
+    Sail.write_reg op_a (Word.toBitVec64 #v[Main[39], Main[40], Main[41] * 65535, Main[41] * 65535])
     pure RETIRE_SUCCESS
 
 attribute [simp] bind StateT.bind ExceptT.bind EStateM.bind ExceptT.bindCont get getThe MonadStateOf.get StateT.get EStateM.get pure StateT.pure ExceptT.pure EStateM.pure Functor.map StateT.map ExceptT.map EStateM.map modify modifyGet EStateM.modifyGet StateT.modifyGet MonadStateOf.modifyGet liftM monadLift MonadLift.monadLift ExceptT.lift StateT.lift ExceptT.mk StateT.run ExceptT.run EStateM.run Sail.SailME.run
 
-set_option debug.skipKernelTC true in
-set_option maxHeartbeats 20000000 in
+-- attribute [-simp] Sail.wX_bits_eq_writeReg
+
+-- set_option debug.skipKernelTC true in
+set_option maxHeartbeats 4000000 in
+set_option pp.proofs false in
+set_option diagnostics false in
 theorem correct
   (Main : Vector (Fin BB) 44)
   (s : SailState)
@@ -99,28 +149,18 @@ theorem correct
     simp [constraints, AddressOperation.constraints, SP1Constraint.toProp, List.Forall, h_is_lw, h_not_lwu, Opcode.ofNat, ByteOpcode.ofNat, Nat.beq, Nat.ble, sub_eq_zero] at cstrs
     obtain ⟨addr_add_cstrs, addr_cstr0, addr_cstr1, addr_cstr2, msb_cstrs, cpu_cstrs, reader_cstrs, chip_cstrs⟩ := cstrs
 
-    have h_op_a_is_reg : Main[6] < 32 :=
-      by
-        simp [ITypeReader.constraints, SP1Constraint.toProp, List.Forall, h_is_lw, h_not_lwu, Opcode.ofNat, ByteOpcode.ofNat, Nat.beq, Nat.ble] at reader_cstrs
-        simp_all only
+    simp [ITypeReader.constraints, SP1Constraint.toProp, List.Forall, Opcode.ofNat, ByteOpcode.ofNat, Nat.ble, Nat.beq] at reader_cstrs
+
+    have h_op_a_is_reg : Main[6]$ < 32 := by simp_all only
     simp [h_op_a_is_reg] at h_read_op_a
-    have h_op_b_is_reg : Main[14] < 32 :=
-      by
-        simp [ITypeReader.constraints, SP1Constraint.toProp, List.Forall, h_is_lw, h_not_lwu, Opcode.ofNat, ByteOpcode.ofNat, Nat.beq, Nat.ble] at reader_cstrs
-        simp_all only
+    have h_op_b_is_reg : Main[14]$ < 32 := by simp_all only
     simp [h_op_b_is_reg] at h_read_op_b
     -- simp [-Word.add_toBitVec64_mod4, ←BitVec.ofNatLT_eq_ofNat (w := 5) (n := Main[14].val) h_op_b_is_reg, h_read_op_b] at h_trusted_read
-    rw [←BitVec.ofNatLT_eq_ofNat (w := 5) (n := Main[14].val) h_op_b_is_reg, h_read_op_b, Option.get!_some] at h_trusted_read
+    rw [←BitVec.ofNatLT_eq_ofNat (w := 5) (n := Main[14]$.val) h_op_b_is_reg, h_read_op_b, Option.get!_some] at h_trusted_read
 
-    cases addr_cstr0
-    · sorry
+    have h_mem_read_is_u64 : Word.isU64 #v[Main[29]$, Main[30]$, Main[31]$, Main[32]$] := by simp_all only [chip_cstrs]
 
-    rename_i h_has_shift
-    simp [h_has_shift] at chip_cstrs h_read_mem addr_cstr2
-
-    have h_mem_read_is_u64 : Word.isU64 #v[Main[29], Main[30], Main[31], Main[32]] := by simp_all only [chip_cstrs]
-
-    have h_over_addr : Main[26] ≠ 0 ∨ Main[27] ≠ 0 :=
+    have h_over_addr : Main[26]$ ≠ 0 ∨ Main[27]$ ≠ 0 :=
       by
         by_contra!
         clear * - addr_cstr1 this
@@ -128,26 +168,12 @@ theorem correct
         simp [h_limb1_0, h_limb2_0] at addr_cstr1
     simp [not_and_or.mpr h_over_addr] at h_read_mem
     obtain ⟨h_read_limb0, h_read_limb1, h_read_limb2, h_read_limb3⟩ := h_read_mem
-    
-    simp [spec_lw, execute_LOAD]
 
-    simp [Sail.readReg, PreSail.readReg, h_read_pc]
-
-    simp [Sail.assert, PreSail.assert, LeanRV64IM.Functions.xlen_bytes]
-
-    simp [vmem_read]
-    simp [ext_data_get_addr]
-    simp [op_b, sp1_op_b]
-
-    simp [Sail.writeReg, PreSail.writeReg, Sail.rX_bits_eq_get_reg?_no_run, h_read_op_b, Option.elim, Option.toSailM]
-
-    simp [check_misaligned, LeanRV64IM.Functions.plat_enable_misaligned_access, LeanRV64IM.Functions.not]
-
-    have h_op_c_is_signExtend : Word.toBitVec64 #v[Main[21], Main[22], Main[23], Main[24]] = BitVec.signExtend 64 (BitVec.ofNat 12 Main[21].val) := by
+    have h_op_c_is_signExtend : Word.toBitVec64 #v[Main[21]$, Main[22]$, Main[23]$, Main[24]$] = BitVec.signExtend 64 (BitVec.ofNat 12 Main[21]$.val) := by
       simp [constraints, AddressOperation.constraints, AddrAddOperation.constraints, CPUState.constraints, ITypeReader.constraints, SP1Constraint.toProp, List.Forall, h_is_lw, h_not_lwu, Opcode.ofNat, ByteOpcode.ofNat, Nat.beq, Nat.ble] at cstrs
       simp_all only
 
-    have h_is_aligned : is_aligned_vaddr (virtaddr.Virtaddr (Word.toBitVec64 #v[Main[15], Main[16], Main[17], Main[18]] + sign_extend op_c)) 4 = true := by
+    have h_is_aligned : is_aligned_vaddr (virtaddr.Virtaddr (Word.toBitVec64 #v[Main[15]$, Main[16]$, Main[17]$, Main[18]$] + BitVec.signExtend 64 op_c)) 4 = true := by
       unfold is_aligned_vaddr
       simp only [op_b, op_c, sp1_op_b, sp1_imm, sign_extend, Sail.BitVec.signExtend]
       rw [h_op_c_is_signExtend] at h_trusted_read
@@ -159,138 +185,185 @@ theorem correct
       -- praise Confucius this works
       bv_omega
 
-    simp [h_is_aligned, split_misaligned, bits_of_virtaddr]
-
-    simp [untilFuelM, untilFuelM.go, Sail.assert, PreSail.assert]
-
-    simp [translateAddr]
-    simp [Sail.readReg, PreSail.readReg, Std.ExtDHashMap.get?_insert, h_mstatus, h_priv]
-    simp [effectivePrivilege, _get_Mstatus_MPRV, Sail.BitVec.extractLsb, translationMode]
-
-    -- clear * - h_mstatus h_priv mem0 mem1 mem2 mem3
-
-    simp [ITypeReader.constraints, SP1Constraint.toProp, List.Forall, Opcode.ofNat, ByteOpcode.ofNat, Nat.ble, Nat.beq] at reader_cstrs
-    obtain ⟨h_add_addr_limb0, h_add_addr_limb1, h_add_addr_limb2, h_addr_add_spec⟩ :=
-      AddrAddOperation.correct
-      _ _ _ _ (by simp)
-      addr_add_cstrs
-      (by simp_all only [reader_cstrs])
-      (Word.isU64_of_cases _
-        (by simp; show Main[21] < 65536; simp_all only [reader_cstrs]) 
-        (by simp; show Main[22] < 65536; simp_all only [reader_cstrs]) 
-        (by simp; show Main[23] < 65536; simp_all only [reader_cstrs]) 
-        (by simp; show Main[24] < 65536; simp_all only [reader_cstrs]))
-      (by sorry) -- TODO(gzgz): not exceeding memory bounds, this should come from trusted_instr
-    simp at h_add_addr_limb0 h_add_addr_limb1 h_add_addr_limb2 h_addr_add_spec
-
-    -- TODO(gzgz): this will come from the cursed mod thingy
-    have h_addr_limb0_ge4 : Main[25] >= 4 :=
-      by
-        by_contra!
-        convert_to Main[25].val < 4 at this
-        simp [Fin.lt_def, Fin.mul_def, Fin.sub_def] at addr_cstr2
-        interval_cases Main[25].val
-        <;> simp at addr_cstr2
-
-    obtain ⟨h_limb2_mem0, h_limb2_mem1⟩ := h_read_limb2
-    have h_read_mem0 : s.mem[(Word.toBitVec64 #v[Main[15], Main[16], Main[17], Main[18]] + sign_extend op_c).toNat]? = some (BitVec.truncate 8 (BitVec.ofNat 16 ↑Main[31])) := by
-      simp only [op_c, sp1_imm, sign_extend, Sail.BitVec.signExtend]
-      rw [←h_op_c_is_signExtend]
-      rw [←h_addr_add_spec]
-      clear * - h_limb2_mem0 h_add_addr_limb0 h_add_addr_limb1 h_add_addr_limb2 h_addr_limb0_ge4
-      simp [-BitVec.toNat_ofNat, Word.toBitVec64, Word.toNat]
-      rw [←BitVec.ofNatLT_eq_ofNat (by omega)]
-      simp [BitVec.ofNatLT_toNat]
-      simp [Word.toNat] at h_limb2_mem0
-      simp [Fin.sub_val_of_le h_addr_limb0_ge4] at h_limb2_mem0
-      rw [←h_limb2_mem0]
-      apply congrArg
-      apply Eq.symm
-      calc 
-        _ = 4 + (↑Main[25] - 4 + _ + _) := by rw [add_comm (b := 4)]
-        _ = 4 + (↑Main[25] - 4) + _ + _ := by rw [←add_assoc, ←add_assoc]
-        _ = ↑Main[25] - 4 + 4 + _ + _ := by rw [add_comm (a := 4)]
-        _ = ↑Main[25] + 4 - 4 + _ + _ := by rw [←Nat.sub_add_comm (k := 4) h_addr_limb0_ge4]
-        _ = ↑Main[25] + (4 - 4) + _ + _ := by rw [Nat.add_sub_assoc (by simp)]
-        _ = ↑Main[25] + ↑Main[26] * 65536 + ↑Main[27] * 4294967296 := by simp
-
-    have h_read_mem1 : s.mem[(Word.toBitVec64 #v[Main[15], Main[16], Main[17], Main[18]] + sign_extend op_c).toNat + 1]? = some (BitVec.truncate 8 ((BitVec.ofNat 16 ↑Main[31]) >>> 8)) := by
-      simp only [op_c, sp1_imm, sign_extend, Sail.BitVec.signExtend]
-      rw [←h_op_c_is_signExtend]
-      rw [←h_addr_add_spec]
-      clear * - h_limb2_mem1 h_add_addr_limb0 h_add_addr_limb1 h_add_addr_limb2 h_addr_limb0_ge4
-      simp [-BitVec.toNat_ofNat, Word.toBitVec64, Word.toNat]
-      rw [←BitVec.ofNatLT_eq_ofNat (by omega)]
-      simp [BitVec.ofNatLT_toNat]
-      simp [Word.toNat] at h_limb2_mem1
-      simp [Fin.sub_val_of_le h_addr_limb0_ge4] at h_limb2_mem1
-      rw [←h_limb2_mem1]
-      apply congrArg
-      apply Eq.symm
-      sorry
-
-    have h_read_mem2 : s.mem[(Word.toBitVec64 #v[Main[15], Main[16], Main[17], Main[18]] + sign_extend op_c).toNat + 2]? = some (BitVec.truncate 8 ((BitVec.ofNat 16 ↑Main[32]))) := by sorry
-
-    have h_read_mem3 : s.mem[(Word.toBitVec64 #v[Main[15], Main[16], Main[17], Main[18]] + sign_extend op_c).toNat + 3]? = some (BitVec.truncate 8 (((BitVec.ofNat 16 ↑Main[32])) >>> 8)) := by sorry
-
-    have h_limb2_is_u16 : Main[31].val < 2^16 := h_mem_read_is_u64 2
-    have h_limb3_is_u16 : Main[32].val < 2^16 := h_mem_read_is_u64 3
-    simp only [←BitVec.ofNatLT_eq_ofNat h_limb2_is_u16, ←BitVec.ofNatLT_eq_ofNat h_limb3_is_u16] at h_read_mem0 h_read_mem1 h_read_mem2 h_read_mem3
-
-    have h_always_within_ram : within_phys_mem (physaddr.Physaddr (Word.toBitVec64 #v[Main[15], Main[16], Main[17], Main[18]] + sign_extend op_c)) 4 = pure true := by
-      sorry
-
-    -- TODO(gzgz): comes from chip_cstrs
     have h_op_a_not_x0 : op_a ≠ 0#5 := by
       simp [op_a, sp1_op_a, BitVec.ofNatLT, BitVec.ofNat]
       have h_imm_c_is_0 : Main[13] = 0 := by simp_all only [chip_cstrs]
-      have h_imm_c_iff_op_a_x0 : Main[13] = 1 ↔ Main[6] = 0 := by simp_all only [reader_cstrs]
+      have h_imm_c_iff_op_a_x0 : Main[13] = 1 ↔ Main[6] = 0 := by
+        simp_all only [reader_cstrs]
       rw [Fin.mk_eq_mk]
       simp
       clear * - h_imm_c_is_0 h_imm_c_iff_op_a_x0
       aesop
+    simp [op_a, sp1_op_a] at h_op_a_not_x0
 
-    simp [-BitVec.toNat_add, mem_read, Sail.readReg, PreSail.readReg, Std.ExtDHashMap.get?_insert, h_mstatus, h_priv, effectivePrivilege, _get_Mstatus_MPRV, Sail.BitVec.extractLsb, translationMode, mem_read_priv, mem_read_priv_meta, checked_mem_read, phys_access_check, bits_of_virtaddr, LeanRV64IM.Functions.sys_pmp_count, within_mmio_readable, get_config_rvfi, Sail.BitVec.addInt, zero_extend, Sail.BitVec.zeroExtend, h_always_within_ram, ext_check_phys_mem_read, phys_mem_read, read_kind_of_flags, read_ram, Sail.sail_mem_read, PreSail.sail_mem_read, PreSail.readBytes, PreSail.readByte, h_read_mem0, h_read_mem1, h_read_mem2, h_read_mem3, MemoryOpResult_drop_meta, h_op_a_not_x0]
-
-    simp [misaligned_order, sys_misaligned_order_decreasing, extend_value, sign_extend, Sail.BitVec.signExtend]
-
-    simp [op_a] at h_op_a_not_x0
-    simp [sp1_lw, Sail.writeReg, PreSail.writeReg, Sail.write_reg, h_op_a_not_x0]
-
-    simp [Word.toBitVec64, Word.toNat]
-
-    have h_correct_limb0 : Main[39] = Main[31] := by simp_all only [chip_cstrs]
-    have h_correct_limb1 : Main[40] = Main[32] := by simp_all only [chip_cstrs]
-    rw [h_correct_limb0, h_correct_limb1]
-
-    have h_pc0 : Main[3].val < 65536 := by show Main[3] < 65536; simp_all only [reader_cstrs]
-    have h_pc1 : Main[4].val < 65536 := by show Main[4] < 65536; simp_all only [reader_cstrs]
-    have h_pc2 : Main[5].val < 65536 := by show Main[5] < 65536; simp_all only [reader_cstrs]
-
-    have h_pc_is_u64 : Main[3].val + Main[4].val * 65536 + Main[5].val * 4294967296 < 2^64 := by
+    have h_pc0 : Main[3]$.val < 65536 := by show Main[3] < 65536; simp_all only [reader_cstrs]
+    have h_pc1 : Main[4]$.val < 65536 := by show Main[4] < 65536; simp_all only [reader_cstrs]
+    have h_pc2 : Main[5]$.val < 65536 := by show Main[5] < 65536; simp_all only [reader_cstrs]
+    have h_pc_is_u64 : Main[3]$.val + Main[4]$.val <<< 16 + Main[5]$.val <<< 32 < 2^64 := by
       simp
       clear * - h_pc0 h_pc1 h_pc2
       omega
-    rw [←BitVec.ofNatLT_eq_ofNat h_pc_is_u64]
-    simp [BitVec.add_def]
 
-    have : (↑(Main[3] + 4) + ↑Main[4] * 65536 + ↑Main[5] * 4294967296 : ℕ) = ↑Main[3] + ↑Main[4] * 65536 + ↑Main[5] * 4294967296 + 4 := by
-      simp [Fin.add_def]
-      rw [Nat.mod_eq_of_lt (by clear * - h_pc0; linarith)]
-      ring_nf
-    rw [this]
-    clear this
-    apply congrArg
+    cases addr_cstr0
+    · sorry
 
-    simp [bitVecToRegidxVal]
-    simp [Sail.BitVec.updateSubrange, Sail.BitVec.updateSubrange', default]
-    sorry
+    · rename_i h_shift
+      simp [h_shift] at chip_cstrs h_read_limb0 h_read_limb1 h_read_limb2 h_read_limb3 addr_cstr2
 
-lemma isprime : Nat.Prime 2013265921 := by native_decide
+      obtain ⟨h_add_addr_limb0, h_add_addr_limb1, h_add_addr_limb2, h_addr_add_spec⟩ :=
+        AddrAddOperation.correct
+        _ _ _ _ (by simp)
+        addr_add_cstrs
+        (by simp_all only [reader_cstrs])
+        (Word.isU64_of_cases _
+          (by clear * - reader_cstrs; simp; show Main[21] < 65536; simp_all only [reader_cstrs])
+          (by clear * - reader_cstrs; simp; show Main[22] < 65536; simp_all only [reader_cstrs])
+          (by clear * - reader_cstrs; simp; show Main[23] < 65536; simp_all only [reader_cstrs])
+          (by clear * - reader_cstrs; simp; show Main[24] < 65536; simp_all only [reader_cstrs])
+          )
+        (by sorry) -- TODO(gzgz): not exceeding memory bounds, this should come from trusted_instr
+      simp at h_add_addr_limb0 h_add_addr_limb1 h_add_addr_limb2 h_addr_add_spec
+      clear reader_cstrs
 
-instance : Lean.Grind.NoNatZeroDivisors (ZMod 2013265921) where
-  no_nat_zero_divisors := by
-    sorry
+      let h_addr_limb0_ge4 : Main[25]$ >= 4 :=
+        by
+          clear * - addr_cstr2
+          by_contra!
+          convert_to Main[25].val < 4 at this
+          simp [Fin.lt_def, Fin.mul_def, Fin.sub_def] at addr_cstr2
+          interval_cases Main[25].val
+          <;> simp at addr_cstr2
+
+      obtain ⟨h_limb2_mem0, h_limb2_mem1⟩ := h_read_limb2
+      obtain ⟨h_limb3_mem2, h_limb3_mem3⟩ := h_read_limb3
+      have h_read_mem0 : s.mem[(Word.toBitVec64 #v[Main[15]$, Main[16]$, Main[17]$, Main[18]$] + signExtend 64 op_c).toNat]? = some (BitVec.truncate 8 (BitVec.ofNat 16 ↑Main[31]$)) := by
+        simp only [op_c, sp1_imm, sign_extend, Sail.BitVec.signExtend]
+        rw [←h_op_c_is_signExtend]
+        rw [←h_addr_add_spec]
+        clear * - h_limb2_mem0 h_add_addr_limb0 h_add_addr_limb1 h_add_addr_limb2 h_addr_limb0_ge4
+        simp [-BitVec.toNat_ofNat, Word.toBitVec64, Word.toNat]
+        rw [←BitVec.ofNatLT_eq_ofNat (by omega)]
+        simp [BitVec.ofNatLT_toNat]
+        simp [Word.toNat] at h_limb2_mem0
+        simp [Fin.sub_val_of_le h_addr_limb0_ge4] at h_limb2_mem0
+        rw [←h_limb2_mem0]
+        apply congrArg
+        apply Eq.symm
+        calc 
+          _ = 4 + (↑Main[25] - 4 + _ + _) := by rw [add_comm (b := 4)]
+          _ = 4 + (↑Main[25] - 4) + _ + _ := by rw [←add_assoc, ←add_assoc]
+          _ = ↑Main[25] - 4 + 4 + _ + _ := by rw [add_comm (a := 4)]
+          _ = ↑Main[25] + 4 - 4 + _ + _ := by rw [←Nat.sub_add_comm (k := 4) h_addr_limb0_ge4]
+          _ = ↑Main[25] + (4 - 4) + _ + _ := by rw [Nat.add_sub_assoc (by simp)]
+          _ = ↑Main[25] + _ + _ := by simp
+
+      have h_read_mem1 : s.mem[(Word.toBitVec64 #v[Main[15]$, Main[16]$, Main[17]$, Main[18]$] + signExtend 64 op_c).toNat + 1]? = some (BitVec.truncate 8 ((BitVec.ofNat 16 ↑Main[31]$) >>> 8)) := by
+        simp only [op_c, sp1_imm, sign_extend, Sail.BitVec.signExtend]
+        rw [←h_op_c_is_signExtend]
+        rw [←h_addr_add_spec]
+        clear * - h_limb2_mem1 h_add_addr_limb0 h_add_addr_limb1 h_add_addr_limb2 h_addr_limb0_ge4
+        simp [-BitVec.toNat_ofNat, Word.toBitVec64, Word.toNat]
+        rw [←BitVec.ofNatLT_eq_ofNat (by omega)]
+        simp [BitVec.ofNatLT_toNat]
+        simp [Word.toNat] at h_limb2_mem1
+        simp [Fin.sub_val_of_le h_addr_limb0_ge4] at h_limb2_mem1
+        rw [←h_limb2_mem1]
+        apply congrArg
+        apply Eq.symm
+        calc 
+          _ = 5 + (↑Main[25] - 4 + _ + _) := by rw [add_comm]
+          _ = 5 + (↑Main[25] - 4) + _ + _ := by rw [←add_assoc, ←add_assoc]
+          _ = ↑Main[25] - 4 + 5 + _ + _ := by rw [add_comm (a := 5)]
+          _ = ↑Main[25] + 5 - 4 + _ + _ := by rw [←Nat.sub_add_comm (k := 4) h_addr_limb0_ge4]
+          _ = ↑Main[25] + (5 - 4) + _ + _ := by rw [Nat.add_sub_assoc (by simp)]
+          _ = ↑Main[25] + 1 + ↑Main[26] <<< 16 + ↑Main[27] <<< 32 := by simp
+          _ = ↑Main[25] + ↑Main[26] <<< 16 + ↑Main[27] <<< 32 + 1 := by ring_nf
+
+      have h_read_mem2 : s.mem[(Word.toBitVec64 #v[Main[15]$, Main[16]$, Main[17]$, Main[18]$] + signExtend 64 op_c).toNat + 2]? = some (BitVec.truncate 8 ((BitVec.ofNat 16 ↑Main[32]$))) := by
+        simp only [op_c, sp1_imm, sign_extend, Sail.BitVec.signExtend]
+        rw [←h_op_c_is_signExtend]
+        rw [←h_addr_add_spec]
+        clear * - h_limb3_mem2 h_add_addr_limb0 h_add_addr_limb1 h_add_addr_limb2 h_addr_limb0_ge4
+        simp [-BitVec.toNat_ofNat, Word.toBitVec64, Word.toNat]
+        rw [←BitVec.ofNatLT_eq_ofNat (by omega)]
+        simp [BitVec.ofNatLT_toNat]
+        simp [Word.toNat] at h_limb3_mem2
+        simp [Fin.sub_val_of_le h_addr_limb0_ge4] at h_limb3_mem2
+        rw [←h_limb3_mem2]
+        apply congrArg
+        apply Eq.symm
+        calc 
+          _ = 6 + (↑Main[25] - 4 + _ + _) := by rw [add_comm]
+          _ = 6 + (↑Main[25] - 4) + _ + _ := by rw [←add_assoc, ←add_assoc]
+          _ = ↑Main[25] - 4 + 6 + _ + _ := by rw [add_comm (a := 6)]
+          _ = ↑Main[25] + 6 - 4 + _ + _ := by rw [←Nat.sub_add_comm (k := 4) h_addr_limb0_ge4]
+          _ = ↑Main[25] + (6 - 4) + _ + _ := by rw [Nat.add_sub_assoc (by simp)]
+          _ = ↑Main[25] + 2 + ↑Main[26] <<< 16 + ↑Main[27] <<< 32 := by simp
+          _ = ↑Main[25] + ↑Main[26] <<< 16 + ↑Main[27] <<< 32 + 2 := by ring_nf
+
+      have h_read_mem3 : s.mem[(Word.toBitVec64 #v[Main[15]$, Main[16]$, Main[17]$, Main[18]$] + signExtend 64 op_c).toNat + 3]? = some (BitVec.truncate 8 (((BitVec.ofNat 16 ↑Main[32]$)) >>> 8)) := by
+        simp only [op_c, sp1_imm, sign_extend, Sail.BitVec.signExtend]
+        rw [←h_op_c_is_signExtend]
+        rw [←h_addr_add_spec]
+        clear * - h_limb3_mem3 h_add_addr_limb0 h_add_addr_limb1 h_add_addr_limb2 h_addr_limb0_ge4
+        simp [-BitVec.toNat_ofNat, Word.toBitVec64, Word.toNat]
+        rw [←BitVec.ofNatLT_eq_ofNat (by omega)]
+        simp [BitVec.ofNatLT_toNat]
+        simp [Word.toNat] at h_limb3_mem3
+        simp [Fin.sub_val_of_le h_addr_limb0_ge4] at h_limb3_mem3
+        rw [←h_limb3_mem3]
+        apply congrArg
+        apply Eq.symm
+        calc 
+          _ = 7 + (↑Main[25] - 4 + _ + _) := by rw [add_comm]
+          _ = 7 + (↑Main[25] - 4) + _ + _ := by rw [←add_assoc, ←add_assoc]
+          _ = ↑Main[25] - 4 + 7 + _ + _ := by rw [add_comm (a := 7)]
+          _ = ↑Main[25] + 7 - 4 + _ + _ := by rw [←Nat.sub_add_comm (k := 4) h_addr_limb0_ge4]
+          _ = ↑Main[25] + (7 - 4) + _ + _ := by rw [Nat.add_sub_assoc (by simp)]
+          _ = ↑Main[25] + 3 + ↑Main[26] <<< 16 + ↑Main[27] <<< 32 := by simp
+          _ = ↑Main[25] + ↑Main[26] <<< 16 + ↑Main[27] <<< 32 + 3 := by ring_nf
+
+      have h_limb2_is_u16 : Main[31]$.val < 2^16 := h_mem_read_is_u64 2
+      have h_limb3_is_u16 : Main[32]$.val < 2^16 := h_mem_read_is_u64 3
+      simp only [←BitVec.ofNatLT_eq_ofNat h_limb2_is_u16, ←BitVec.ofNatLT_eq_ofNat h_limb3_is_u16] at h_read_mem0 h_read_mem1 h_read_mem2 h_read_mem3
+
+      simp [-BitVec.toNat_add, spec_lw, execute_LOAD, Sail.readReg, PreSail.readReg, h_read_pc, Sail.assert, PreSail.assert,
+           LeanRV64IM.Functions.xlen_bytes, vmem_read, ext_data_get_addr, op_b, sp1_op_b, Sail.writeReg,
+           PreSail.writeReg, Sail.rX_bits_eq_get_reg?_no_run, h_read_op_b, Option.elim, Option.toSailM,
+           check_misaligned, LeanRV64IM.Functions.plat_enable_misaligned_access, LeanRV64IM.Functions.not,
+           h_is_aligned, split_misaligned, bits_of_virtaddr, untilFuelM, untilFuelM.go, Sail.assert, PreSail.assert,
+           translateAddr, Std.ExtDHashMap.get?_insert, h_mstatus, h_priv, effectivePrivilege, _get_Mstatus_MPRV,
+           Sail.BitVec.extractLsb, translationMode, mem_read, Sail.readReg, PreSail.readReg, Sail.BitVec.extractLsb,
+           translationMode, mem_read_priv, mem_read_priv_meta, checked_mem_read, phys_access_check, bits_of_virtaddr,
+           LeanRV64IM.Functions.sys_pmp_count, within_mmio_readable, get_config_rvfi, Sail.BitVec.addInt, zero_extend,
+           Sail.BitVec.zeroExtend, within_phys_mem, ext_check_phys_mem_read, phys_mem_read, read_kind_of_flags,
+           read_ram, Sail.sail_mem_read, PreSail.sail_mem_read, PreSail.readBytes, PreSail.readByte, h_read_mem0,
+           h_read_mem1, h_read_mem2, h_read_mem3, MemoryOpResult_drop_meta, h_op_a_not_x0, misaligned_order,
+           sys_misaligned_order_decreasing, extend_value, sign_extend, Sail.BitVec.signExtend, sp1_lw, op_a, sp1_op_a,
+           Sail.run_write_reg_no_run, h_op_a_not_x0]
+
+      have h_correct_limb0 : Main[39]$ = Main[31]$ := by simp_all only [chip_cstrs]
+      have h_correct_limb1 : Main[40]$ = Main[32]$ := by simp_all only [chip_cstrs]
+      rw [h_correct_limb0, h_correct_limb1]
+
+      -- nextPC write
+      simp [Word.toBitVec64, Word.toNat]
+      rw [←BitVec.ofNatLT_eq_ofNat h_pc_is_u64]
+      simp [BitVec.add_def]
+      have : (↑(Main[3]$ + 4) + ↑Main[4]$ <<< 16 + ↑Main[5]$ <<< 32 : ℕ) = ↑Main[3]$ + ↑Main[4]$ <<< 16 + ↑Main[5]$ <<< 32 + 4 := by
+        simp [Fin.add_def]
+        rw [Nat.mod_eq_of_lt (by clear * - h_pc0; linarith)]
+        ring_nf
+      rw [this]
+      clear this
+      simp [op_a]
+
+      apply congrArg
+      apply congrArg
+
+      -- op_a/rd write
+      simp [Sail.BitVec.updateSubrange, Sail.BitVec.updateSubrange', default]
+      sorry
 
 lemma helper2
   {x : Fin BB}
